Fomega/Basic/Derivations.lean
@@ -8,28 +8,6 @@ import Fomega.Basic.Classification
 
 namespace Fomega
 
-  -- A, B ⊢ (X : ★) -> (A -> B -> X) -> X
-  @[simp]
-  def PairTy (A B : Term) : Term := .all mf ★ (.all mf
-    (.all mf A (.all mf B (.bound .kind 2)))
-    (.bound .kind 0))
-
-  -- A, B, a, b ⊢ λ X : ★. λ ctor : (A -> B -> X). ctor a b
-  @[simp]
-  def pair (A B a b : Term) : Term := .lam mf ★
-    (.lam mf (.all mf A (.all mf B (.bound .kind 2)))
-      (.app mf (.app mf (.bound .type 0) a) b))
-
-  -- A B p ⊢ p A (λ a b. a)
-  @[simp]
-  def fst (A B p : Term) : Term := .app mf
-    (.app mf p A)
-    (.lam mf A (.lam mf B (.bound .type 1)))
-
-  -- A B p ⊢ p A (λ a b. b)
-  @[simp]
-  def snd (A B p : Term) : Term := p `@f A `@f (.lam mf A (.lam mf B (.bound .type 0)))
-
   -- ⊢ (X : ★) -> X -> X
   @[simp]
   def IdTy : Term := .all mf ★ (.all mf (.bound .kind 0) (.bound .kind 1))
