Fomega/Basic/Substitution.lean
@@ -82,6 +82,17 @@ namespace Fomega.Proof
   case app _j1 _j2 j3 ih1 ih2 =>
     simp; constructor; apply ih1 h2 h3 j2; apply ih2 h2 h3 j2
     subst j3; simp
+  case prod ih1 ih2 =>
+    simp; constructor; apply ih1 h2 h3 j2; apply ih2 h2 h3 j2
+  case pair ih1 ih2 ih3 ih4 =>
+    simp; constructor; apply ih1 h2 h3 j2; apply ih2 h2 h3 j2
+    apply ih3 h2 h3 j2; apply ih4 h2 h3 j2
+  case fst ih =>
+    simp; constructor; apply ih h2 h3 j2
+  case snd ih =>
+    simp; constructor; apply ih h2 h3 j2
+  case id ih =>
+    simp; apply Judgment.id; apply ih h2 h3 j2
   case conv Γ' t' A' B K _j1 _j2 j3 ih1 ih2 =>
     constructor; apply ih1 h2 h3 j2; apply ih2 h2 h3 j2
     apply RedConv.subst _ j3
