Fomega/Parametricity.lean
@@ -1,53 +1,53 @@
 
-import Common
-import Fomega.Proof
+-- import Common
+-- import Fomega.Proof
 
-namespace Fomega.Proof
+-- namespace Fomega.Proof
 
-  def Tuple (n : Nat) (T : (i : Nat) -> i < n -> Type) : Type := (i : Nat) -> (b : i < n) -> T i b
+--   def Tuple (n : Nat) (T : (i : Nat) -> i < n -> Type) : Type := (i : Nat) -> (b : i < n) -> T i b
 
-  abbrev RelCtx n := Tuple n (λ _ _ => Ctx)
-  abbrev RelKind n (Γ : RelCtx n) := Tuple n (λ i b => Σ' (t : Term), (t ⊢ Γ i b ∧ Γ i b ⊢ t : □))
+--   abbrev RelCtx n := Tuple n (λ _ _ => Ctx)
+--   abbrev RelKind n (Γ : RelCtx n) := Tuple n (λ i b => Σ' (t : Term), (t ⊢ Γ i b ∧ Γ i b ⊢ t : □))
 
-  -- abbrev rel_kinds n Γ : RelKind n Γ := λ _ _ => PSigma.mk □ (by sorry)
-  -- abbrev rel_types n Γ : RelKind n Γ := λ _ _ => PSigma.mk ★ (by sorry)
+--   -- abbrev rel_kinds n Γ : RelKind n Γ := λ _ _ => PSigma.mk □ (by sorry)
+--   -- abbrev rel_types n Γ : RelKind n Γ := λ _ _ => PSigma.mk ★ (by sorry)
 
-  abbrev RelType n Γ (k : RelKind n Γ) := Tuple n (λ i b => Σ' (t : Term), (t ⊢ Γ i b ∧ Γ i b ⊢ t : (k i b).1))
+--   abbrev RelType n Γ (k : RelKind n Γ) := Tuple n (λ i b => Σ' (t : Term), (t ⊢ Γ i b ∧ Γ i b ⊢ t : (k i b).1))
 
-  abbrev RelTerm n Γ (k : RelKind n Γ) (φ : RelType n Γ k) := Tuple n (λ i b => Σ' (t : Term), (t ⊢ (Γ i b) ∧ (Γ i b) ⊢ t : (φ i b).1))
+--   abbrev RelTerm n Γ (k : RelKind n Γ) (φ : RelType n Γ k) := Tuple n (λ i b => Σ' (t : Term), (t ⊢ (Γ i b) ∧ (Γ i b) ⊢ t : (φ i b).1))
 
-  def Rel (n : Nat) Γ (k : RelKind n Γ) (φ : RelType n Γ k) : Type := RelTerm n Γ k φ -> Prop
+--   def Rel (n : Nat) Γ (k : RelKind n Γ) (φ : RelType n Γ k) : Type := RelTerm n Γ k φ -> Prop
 
-  -- abbrev fnTpiType {n : Nat} {Γ : RelCtx n} {k : RelKind n}
-  --   (α : RelType n Γ k) (ty : RelType n (λ i b => (α i b).1 :: (Γ i b)) (rel_types n))
-  --   : RelType n Γ (rel_types n)
-  -- := λ i b => PSigma.mk (.all mf (α i b).1 (ty i b).1) (by {
-  --   apply And.intro; constructor; exact (α i b).2.1; exact (ty i b).2.1
-  --   constructor; exact (α i b).2.2; exact (ty i b).2.2
-  -- })
+--   -- abbrev fnTpiType {n : Nat} {Γ : RelCtx n} {k : RelKind n}
+--   --   (α : RelType n Γ k) (ty : RelType n (λ i b => (α i b).1 :: (Γ i b)) (rel_types n))
+--   --   : RelType n Γ (rel_types n)
+--   -- := λ i b => PSigma.mk (.all mf (α i b).1 (ty i b).1) (by {
+--   --   apply And.intro; constructor; exact (α i b).2.1; exact (ty i b).2.1
+--   --   constructor; exact (α i b).2.2; exact (ty i b).2.2
+--   -- })
 
-  -- def fnTpi {n : Nat} {Γ : RelCtx n} {k : RelKind n}
-  --   (α : RelType n Γ k) (ty : RelType n (λ i b => (α i b).1 :: (Γ i b)) (rel_types n))
-  --   (F : (φ:RelType n Γ k) -> Rel n Γ k φ -> Prop)
-  --   : Rel n Γ (rel_types n) (fnTpiType α ty)
-  -- := λ t => ∀ (s:RelType n Γ k) R,
-  --   F (λ i b => (ty i b).1 β[(s i b).1]) R ->
-  --   R (λ i b => PSigma.mk (.app mf (t i b).1 (s i b))
-  --     (by {
-  --     apply And.intro; constructor; exact (t i b).2.1; exact (h i b).1
-  --     constructor; exact (t i b).2.2; exact (h i b).2; simp
-  --   }))
+--   -- def fnTpi {n : Nat} {Γ : RelCtx n} {k : RelKind n}
+--   --   (α : RelType n Γ k) (ty : RelType n (λ i b => (α i b).1 :: (Γ i b)) (rel_types n))
+--   --   (F : (φ:RelType n Γ k) -> Rel n Γ k φ -> Prop)
+--   --   : Rel n Γ (rel_types n) (fnTpiType α ty)
+--   -- := λ t => ∀ (s:RelType n Γ k) R,
+--   --   F (λ i b => (ty i b).1 β[(s i b).1]) R ->
+--   --   R (λ i b => PSigma.mk (.app mf (t i b).1 (s i b))
+--   --     (by {
+--   --     apply And.intro; constructor; exact (t i b).2.1; exact (h i b).1
+--   --     constructor; exact (t i b).2.2; exact (h i b).2; simp
+--   --   }))
 
-  def KindMap (n:Nat) (Γ : RelCtx n) : Type := Nat -> RelKind n Γ
-  def TypeMap (n:Nat) Γ (k : KindMap n Γ) : Type := Nat -> RelType n Γ (k n)
-  def TermMap (n:Nat) Γ (k : KindMap n Γ) (φ : TypeMap n Γ k) : Type := Nat -> RelTerm n Γ (k n) (φ n)
-
-
-
-  theorem parametricity : ∀ (n : Nat) (Γ : RelCtx n) (Fam : ∀ {n Γ k φ}, Rel n Γ k φ)
-    (ζ : KindMap n Γ) (ξ : TypeMap n Γ ζ) (φ : TermMap n Γ ζ ξ),
-    (∀ i, Fam (φ i)) -> Δ ⊢ t : A -> True
-  := by sorry
+--   def KindMap (n:Nat) (Γ : RelCtx n) : Type := Nat -> RelKind n Γ
+--   def TypeMap (n:Nat) Γ (k : KindMap n Γ) : Type := Nat -> RelType n Γ (k n)
+--   def TermMap (n:Nat) Γ (k : KindMap n Γ) (φ : TypeMap n Γ k) : Type := Nat -> RelTerm n Γ (k n) (φ n)
 
 
-end Fomega.Proof
+
+--   theorem parametricity : ∀ (n : Nat) (Γ : RelCtx n) (Fam : ∀ {n Γ k φ}, Rel n Γ k φ)
+--     (ζ : KindMap n Γ) (ξ : TypeMap n Γ ζ) (φ : TermMap n Γ ζ ξ),
+--     (∀ i, Fam (φ i)) -> Δ ⊢ t : A -> True
+--   := by sorry
+
+
+-- end Fomega.Proof
