Fomega/PreProof.lean
@@ -17,6 +17,11 @@ namespace Fomega
   | all : IsPreProof A -> IsPreProof B -> IsPreProof (.all mf A B)
   | lam : IsPreProof A -> IsPreProof t -> IsPreProof (.lam mf A t)
   | app : IsPreProof f -> IsPreProof a -> IsPreProof (.app mf f a)
+  | prod : IsPreProof A -> IsPreProof B -> IsPreProof (.sprod A B)
+  | pair : IsPreProof a -> IsPreProof b -> IsPreProof (.spair a b)
+  | fst : IsPreProof t -> IsPreProof (.fst t)
+  | snd : IsPreProof t -> IsPreProof (.snd t)
+  | id : IsPreProof t -> IsPreProof (.id t)
 
   namespace IsPreProof
     theorem from_subst : IsPreProof ([σ]t) -> IsPreProof t := by
@@ -30,6 +35,13 @@ namespace Fomega
       constructor; apply ih1 j1; apply ih2 j2
     case _ ih1 ih2 j1 j2 =>
       constructor; apply ih1 j1; apply ih2 j2
+    case _ ih1 ih2 j1 j2 =>
+      constructor; apply ih1 j1; apply ih2 j2
+    case _ ih j => constructor; apply ih j
+    case _ ih j => constructor; apply ih j
+    case _ ih1 ih2 j1 j2 =>
+      constructor; apply ih1 j1; apply ih2 j2
+    case _ ih j => constructor; apply ih j
 
     theorem ren : IsPreProof t -> IsPreProof ([r#r]t) := by
     intro j
@@ -46,6 +58,13 @@ namespace Fomega
       simp at ih2; exact ih2
     case app _j1 _j2 ih1 ih2 =>
       constructor; apply ih1; apply ih2
+    case prod ih1 ih2 =>
+      constructor; apply ih1; apply ih2
+    case pair ih1 ih2 =>
+      constructor; apply ih1; apply ih2
+    case fst ih => constructor; apply ih
+    case snd ih => constructor; apply ih
+    case id ih => constructor; apply ih
 
     theorem lift : (∀ n s, σ n = .replace s -> IsPreProof s) -> ∀ n s, ^σ n = .replace s -> IsPreProof s := by
     intro h n s eq; simp at *
@@ -78,6 +97,13 @@ namespace Fomega
       simp at ih2; exact ih2
     case app _j1 _j2 ih1 ih2 =>
       constructor; apply ih1 h; apply ih2 h
+    case prod ih1 ih2 =>
+      constructor; apply ih1 h; apply ih2 h
+    case pair ih1 ih2 =>
+      constructor; apply ih1 h; apply ih2 h
+    case fst ih => constructor; apply ih h
+    case snd ih => constructor; apply ih h
+    case id ih => constructor; apply ih h
 
     theorem beta : IsPreProof b -> IsPreProof t -> IsPreProof (b β[t]) := by
     simp; intro j1 j2
@@ -95,11 +121,7 @@ namespace Fomega
 
     theorem from_proof : Judgment v Γ ix -> FromProofType v ix := by
     intro j; induction j <;> simp at *
-    case ax => constructor
-    case var => constructor
-    case pi _j1 _j2 ih1 ih2 => constructor; apply ih1; apply ih2
-    case lam j1 _j2 ih1 ih2 => constructor; cases ih1; all_goals simp [*]
-    case app => constructor <;> simp [*]
+    all_goals (try (constructor <;> simp [*]))
     case conv => simp [*]
 
     -- theorem from_proof_type : t ⊢ Γ -> Γ ⊢ t : A -> IsPreProof A := by
