Fomega/Proof.lean
@@ -42,11 +42,30 @@ namespace Fomega
     Judgment .prf Γ (a, A) ->
     B' = (B β[a]) ->
     Judgment .prf Γ (.app mf f a, B')
+  | prod :
+    Judgment .prf Γ (A, ★) ->
+    Judgment .prf Γ (B, ★) ->
+    Judgment .prf Γ (.sprod A B, ★)
+  | pair :
+    Judgment .prf Γ (a, A) ->
+    Judgment .prf Γ (b, B) ->
+    Judgment .prf Γ (A, ★) ->
+    Judgment .prf Γ (B, ★) ->
+    Judgment .prf Γ (.spair a b, .sprod A B)
+  | fst :
+    Judgment .prf Γ (t, .sprod A B) ->
+    Judgment .prf Γ (.fst t, A)
+  | snd :
+    Judgment .prf Γ (t, .sprod A B) ->
+    Judgment .prf Γ (.snd t, B)
   | conv :
     Judgment .prf Γ (t, A) ->
     Judgment .prf Γ (B, .const K) ->
     A =β= B ->
     Judgment .prf Γ (t, B)
+  | id :
+    Judgment .prf Γ (t, A) ->
+    Judgment .prf Γ (.id t, A)
 
   notation:170 Γ:170 " ⊢ " t:170 " : " A:170 => Judgment JudgmentVariant.prf Γ (t, A)
   notation:170 "⊢ " Γ:170 => Judgment JudgmentVariant.wf Γ ()
